prove compiler soundness for exception language
I had to convert the handler address to an optional type so that it is
possible to not have an exception handler, which halts the machine in
case of an exception.

Exception.v
@@ -53,15 +53,17 @@ Fixpoint comp' (x : Expr) (r : nat) (c : Code) : Code :=
 
 Definition comp (x : Expr) : Code := comp' x 0 HALT.
 
+Definition Han := option adr.
+
 Inductive Elem : Set :=
 | NUM : nat -> Elem
-| HAN : Code -> adr -> Elem.
+| HAN : Code -> Han -> Elem.
 
 (** * Virtual Machine *)
 
 Inductive Conf : Type :=
-| conf : Code -> nat -> Mem Elem -> adr -> Conf
-| fail : Mem Elem -> adr -> Conf.
+| conf : Code -> nat -> Mem Elem -> Han -> Conf
+| fail : Mem Elem -> Han -> Conf.
 
 Notation "⟨ x , y , z , p ⟩" := (conf x y z p).
 Notation "⟪ x , y ⟫" := (fail x y).
@@ -72,9 +74,9 @@ Inductive VM : Conf -> Conf -> Prop :=
 | vm_add c s a r n p : get r s = NUM n -> ⟨ADD r c, a , s, p⟩ ==> ⟨c , n + a,  s, p⟩
 | vm_store c s a r p : ⟨STORE r c, a , s, p⟩ ==> ⟨c , a,  set r (NUM a) s, p⟩
 | vm_throw a s p : ⟨THROW, a , s, p⟩ ==> ⟪s, p⟫
-| vm_fail p p' s a c : get p s = HAN c p' -> ⟪s, p⟫ ==> ⟨c, a, s, p'⟩
-| vm_unmark p p' s a c c' : get p s = HAN c' p' -> ⟨UNMARK c, a, s, p⟩ ==> ⟨c, a, s, p'⟩
-| vm_mark p r s a c c' : ⟨MARK r c' c, a, s, p⟩ ==> ⟨c, a, set r (HAN c' p) s, r⟩
+| vm_fail p p' s c : get p s = HAN c p' -> ⟪s, Some p⟫ ==> ⟨c, 0, s, p'⟩
+| vm_unmark p p' s a c c' : get p s = HAN c' p' -> ⟨UNMARK c, a, s, Some p⟩ ==> ⟨c, a, s, p'⟩
+| vm_mark p r s a c c' : ⟨MARK r c' c, a, s, p⟩ ==> ⟨c, a, set r (HAN c' p) s, Some r⟩
 where "x ==> y" := (VM x y).
 
 (** * Calculation *)
@@ -211,24 +213,71 @@ Proof.
      ∪ {a s s', ⟨ comp' e2 r c, 0 , s', p ⟩ | s =[r] s' /\ get r s' = HAN (comp' e2 r c) p /\ P a s /\ eval e1 = None}).
   <== {apply vm_fail}
   ({a s s' n, ⟨ c, n, s', p ⟩ | s =[r] s' /\ get r s' = HAN (comp' e2 r c) p /\ P a s /\ eval e1 = Some n}
-     ∪ {a s s', ⟪ s', r ⟫ | s =[r] s' /\ get r s' = HAN (comp' e2 r c) p /\ P a s /\ eval e1 = None}).
+     ∪ {a s s', ⟪ s', Some r ⟫ | s =[r] s' /\ get r s' = HAN (comp' e2 r c) p /\ P a s /\ eval e1 = None}).
   ⊇ {lemma1}
   ({a s s' n, ⟨ c, n, s', p ⟩ | s =[r] s' /\ get r s' = HAN (comp' e2 r c) p /\ P a s /\ eval e1 = Some n}
-     ∪ {a s s', ⟪ s', r ⟫ | set r (HAN (comp' e2 r c) p) s =[r+1] s' /\ P a s /\ eval e1 = None}).
+     ∪ {a s s', ⟪ s', Some r ⟫ | set r (HAN (comp' e2 r c) p) s =[r+1] s' /\ P a s /\ eval e1 = None}).
   <== {eapply vm_unmark}
-  ({a s s' n, ⟨UNMARK c, n, s', r⟩ | s =[r] s' /\ get r s' = HAN (comp' e2 r c) p /\ P a s /\ eval e1 = Some n}
-     ∪ {a s s', ⟪ s', r⟫ | set r (HAN (comp' e2 r c) p) s =[r+1] s' /\ P a s /\ eval e1 = None}).
+  ({a s s' n, ⟨UNMARK c, n, s', Some r⟩ | s =[r] s' /\ get r s' = HAN (comp' e2 r c) p /\ P a s /\ eval e1 = Some n}
+     ∪ {a s s', ⟪ s', Some r⟫ | set r (HAN (comp' e2 r c) p) s =[r+1] s' /\ P a s /\ eval e1 = None}).
   ⊇ {lemma1}
-    ({a s s' n, ⟨UNMARK c, n, s', r⟩ | set r (HAN (comp' e2 r c) p) s =[r+1] s' /\ P a s /\ eval e1 = Some n}
-     ∪ {a s s', ⟪ s', r⟫ | set r (HAN (comp' e2 r c) p) s =[r+1] s' /\ P a s /\ eval e1 = None}).
+    ({a s s' n, ⟨UNMARK c, n, s', Some r⟩ | set r (HAN (comp' e2 r c) p) s =[r+1] s' /\ P a s /\ eval e1 = Some n}
+     ∪ {a s s', ⟪ s', Some r⟫ | set r (HAN (comp' e2 r c) p) s =[r+1] s' /\ P a s /\ eval e1 = None}).
   ⊇ {eauto}
-    ({a s'' s' n, ⟨UNMARK c, n, s', r⟩ | s'' =[r+1] s' /\ (exists s, set r (HAN (comp' e2 r c) p) s = s'' /\ P a s) /\ eval e1 = Some n}
-     ∪ {a s'' s', ⟪ s', r⟫ | s'' =[r+1] s' /\ (exists s, set r (HAN (comp' e2 r c) p) s = s'' /\ P a s) /\ eval e1 = None}).
+    ({a s'' s' n, ⟨UNMARK c, n, s', Some r⟩ | s'' =[r+1] s' /\ (exists s, set r (HAN (comp' e2 r c) p) s = s'' /\ P a s) /\ eval e1 = Some n}
+     ∪ {a s'' s', ⟪ s', Some r⟫ | s'' =[r+1] s' /\ (exists s, set r (HAN (comp' e2 r c) p) s = s'' /\ P a s) /\ eval e1 = None}).
   <|= {eapply IHe1}
-    ({a s'', ⟨comp' e1 (r+1) (UNMARK c), a , s'', r⟩ | exists s, set r (HAN (comp' e2 r c) p) s = s'' /\ P a s}).
+    ({a s'', ⟨comp' e1 (r+1) (UNMARK c), a , s'', Some r⟩ | exists s, set r (HAN (comp' e2 r c) p) s = s'' /\ P a s}).
   ⊇ {eauto}
-    ({a s, ⟨comp' e1 (r+1) (UNMARK c), a , set r (HAN (comp' e2 r c) p) s, r⟩ | P a s}).
+    ({a s, ⟨comp' e1 (r+1) (UNMARK c), a , set r (HAN (comp' e2 r c) p) s, Some r⟩ | P a s}).
   <== {apply vm_mark}
     ({a s, ⟨MARK r (comp' e2 r c) (comp' e1 (r+1) (UNMARK c)), a , s, p⟩ | P a s}).
   [].
+Qed.
+
+
+
+(* Specialise the spec to singleton sets. *)
+Corollary spec' e r a c s p:
+  exists s', ⟨comp' e r c, a, s, p⟩  =>> match eval e with
+                                         | Some n => ⟨c , n, s', p⟩
+                                         | None => ⟪ s', p⟫
+                                         end /\ s =[r] s' .
+Proof.
+  pose (spec e r c p (fun a' s' => a = a' /\ s = s') (⟨comp' e r c, a, s, p⟩)) as S. simpl in S.
+  premise S. eauto.
+  repeat autodestruct. remember (eval e) as E.
+  destruct E; destruct H; repeat autodestruct;subst; eexists; eauto. 
+Qed.
+
+
+(** * Soundness *)
+  
+(** Since the VM is defined as a small step operational semantics, we *)
+(* have to prove that the VM is deterministic and does not get stuck in *)
+(* order to derive soundness from the above theorem. *)
+
+
+Ltac mem_get := match goal with
+                | [H : get _ _ = _, I : get _ _ = _ |- _] => rewrite H in I; inversion I
+                end.
+
+Lemma determ_vm : determ VM.
+  intros C C1 C2 V. induction V; intro V'; inversion V'; subst; try mem_get; reflexivity.
+Qed.
+
+
+Theorem sound x a s C : ⟨comp x, a, s, None⟩ =>>! C -> exists s', C = match eval x with
+                                                                     | Some n => ⟨HALT, n, s', None⟩
+                                                                     | None => ⟪ s', None⟫
+                                                                     end.
+Proof.
+  intros.
+  pose (spec' x 0 a HALT s None) as H'. repeat autodestruct. unfold comp in *. pose (determ_trc determ_vm) as D.
+  unfold determ in D. remember (eval x) as E. destruct E.
+  eexists. eapply D. apply H. split. apply H0. intro Contra. destruct Contra.
+  inversion H2.
+
+  eexists. eapply D. apply H. split. apply H0. intro Contra. destruct Contra.
+  inversion H2.
 Qed.
